WIP Safe Checker

pcuic/theories/PCUICTyping.v
@@ -689,6 +689,10 @@ Section TypeLocal.
       All_local_env (Γ ,, vdef na b t).
 End TypeLocal.
 
+Arguments localenv_nil {_}.
+Arguments localenv_cons_def {_ _ _ _ _} _ _.
+Arguments localenv_cons_abs {_ _ _ _} _ _.
+
 (** Well-formedness of local environments embeds a sorting for each variable *)
 
 Definition lift_typing (P : global_context -> context -> term -> term -> Type) :
@@ -714,7 +718,7 @@ Section TypeLocalOver.
   Inductive All_local_env_over (Σ : global_context) :
     forall (Γ : context), All_local_env (lift_typing typing Σ) Γ -> Type :=
   | localenv_over_nil :
-      All_local_env_over Σ [] (localenv_nil _)
+      All_local_env_over Σ [] localenv_nil
 
   | localenv_over_cons_abs Γ na t
       (all : All_local_env (lift_typing typing Σ) Γ) :
@@ -722,7 +726,7 @@ Section TypeLocalOver.
       forall (tu : lift_typing typing Σ Γ t None),
         property Σ Γ all _ _ (projT2 tu) ->
         All_local_env_over Σ (Γ ,, vass na t)
-                           (localenv_cons_abs _ Γ na t all tu)
+                           (localenv_cons_abs all tu)
 
   | localenv_over_cons_def Γ na b t
       (all : All_local_env (lift_typing typing Σ) Γ) (tb : typing Σ Γ b t) :
@@ -731,7 +735,7 @@ Section TypeLocalOver.
       forall (tu : lift_typing typing Σ Γ t None),
         property Σ Γ all _ _ (projT2 tu) ->
         All_local_env_over Σ (Γ ,, vdef na b t)
-                           (localenv_cons_def _ Γ na b t all tu tb).
+                           (localenv_cons_def all tu tb).
 End TypeLocalOver.
 
 Section WfArity.
@@ -1204,7 +1208,45 @@ Definition Forall_decls_typing `{checker_flags}
 Lemma refine_type `{checker_flags} Σ Γ t T U : Σ ;;; Γ |- t : T -> T = U -> Σ ;;; Γ |- t : U.
 Proof. now intros Ht ->. Qed.
 
+
 Notation wf_local Σ Γ := (All_local_env (lift_typing typing Σ) Γ).
+
+Section wf_local.
+  Context `{checker_flags}.
+
+  Definition wf_local_rel Σ Γ Γ'
+    := (All_local_env (lift_typing (fun Σ0 Γ0 t T => Σ0 ;;; Γ ,,, Γ0 |- t : T) Σ) Γ').
+
+  Definition wf_local_rel_nil {Σ Γ} : wf_local_rel Σ Γ []
+    := localenv_nil.
+
+  Definition wf_local_rel_abs {Σ Γ Γ' A na} :
+    wf_local_rel Σ Γ Γ' -> {u & Σ ;;; Γ ,,, Γ' |- A : tSort u }
+    -> wf_local_rel Σ Γ (Γ',, vass na A)
+    := localenv_cons_abs.
+
+  Definition wf_local_rel_def {Σ Γ Γ' t A na} :
+    wf_local_rel Σ Γ Γ'
+    -> isType Σ (Γ ,,, Γ') A
+    -> Σ ;;; Γ ,,, Γ' |- t : A
+    -> wf_local_rel Σ Γ (Γ',, vdef na t A)
+    := localenv_cons_def.
+
+  Lemma wf_local_rel_local Σ Γ :
+    wf_local Σ Γ -> wf_local_rel Σ [] Γ.
+  Proof.
+    intro X. eapply All_local_env_impl. exact X.
+    intros Γ0 t [] X0; cbn; rewrite app_context_nil_l; assumption.
+  Defined.
+
+  Lemma wf_local_local_rel Σ Γ :
+    wf_local_rel Σ [] Γ -> wf_local Σ Γ.
+  Proof.
+    intro X. eapply All_local_env_impl. exact X.
+    intros Γ0 t [] XX; cbn in XX; rewrite app_context_nil_l in XX; assumption.
+  Defined.
+
+End wf_local.
 
 Section wf_local_size.
   Context `{checker_flags} (Σ : global_context).
@@ -1522,7 +1564,7 @@ Proof.
   inv wfΣ.
   rename X14 into Xg.
   constructor; auto. unfold Forall_decls_typing in IH.
-  - specialize (IH (existT _ (Σ, φ) (existT _ X13 (existT _ [] (existT _ (localenv_nil (lift_typing typing (Σ, φ))) (existT _ (tSort Universe.type0m ) (existT _ _ (type_Sort _ _ Level.prop (localenv_nil _ ))))))))).
+  - specialize (IH (existT _ (Σ, φ) (existT _ X13 (existT _ [] (existT _ (localenv_nil) (existT _ (tSort Universe.type0m ) (existT _ _ (type_Sort _ _ Level.prop (localenv_nil))))))))).
     simpl in IH. forward IH. constructor 1. simpl. lia.
     apply IH; auto.
   - simpl. simpl in *.
@@ -1531,13 +1573,13 @@ Proof.
       destruct cst_body; simpl in *.
       simpl.
       intros. red in Xg. simpl in Xg.
-      specialize (IH (existT _ (Σ, φ) (existT _ X13 (existT _ _ (existT _ (localenv_nil _) (existT _ _ (existT _ _ Xg))))))).
+      specialize (IH (existT _ (Σ, φ) (existT _ X13 (existT _ _ (existT _ localenv_nil (existT _ _ (existT _ _ Xg))))))).
       simpl in IH.
       forward IH. constructor 1. simpl; lia.
       apply IH.
       red. simpl. red in Xg; simpl in Xg.
       destruct Xg as [s Hs]. red. simpl.
-      specialize (IH (existT _ (Σ, φ) (existT _ X13 (existT _ _ (existT _ (localenv_nil _) (existT _ _ (existT _ _ Hs))))))).
+      specialize (IH (existT _ (Σ, φ) (existT _ X13 (existT _ _ (existT _ localenv_nil (existT _ _ (existT _ _ Hs))))))).
       simpl in IH.
       forward IH. constructor 1. simpl; lia. exists s. eapply IH.
     + red in Xg.
@@ -1562,7 +1604,7 @@ Proof.
          apply IH. simpl. constructor 1. simpl. auto with arith.
       ++ apply (ind_arity_eq Xg).
       ++ apply onArity in Xg. destruct Xg as [s Hs]. exists s; auto.
-         specialize (IH (existT _ (Σ, φ) (existT _ X13 (existT _ _ (existT _ (localenv_nil _) (existT _ _ (existT _ _ Hs))))))).
+         specialize (IH (existT _ (Σ, φ) (existT _ X13 (existT _ _ (existT _ localenv_nil (existT _ _ (existT _ _ Hs))))))).
          simpl in IH. simpl. apply IH; constructor 1; simpl; lia.
       ++ intros Hprojs; pose proof (onProjections Xg Hprojs); auto. simpl in *.
          destruct X14; constructor; auto. eapply Alli_impl; eauto. clear on_projs0. intros.
@@ -1649,15 +1691,15 @@ Proof.
           ** simpl. lia.
 
     -- eapply X5; eauto. simpl in X14.
-       specialize (X14 [] (localenv_nil _) _ _ (type_Sort _ _ Level.prop (localenv_nil _))).
+       specialize (X14 [] localenv_nil _ _ (type_Sort _ _ Level.prop localenv_nil)).
        simpl in X14. forward X14; auto. lia. apply X14.
 
     -- eapply X6; eauto.
-       specialize (X14 [] (localenv_nil _) _ _ (type_Sort _ _ Level.prop (localenv_nil _))).
+       specialize (X14 [] localenv_nil _ _ (type_Sort _ _ Level.prop localenv_nil)).
        simpl in X14. forward X14; auto. lia. apply X14.
 
     -- eapply X7; eauto.
-       specialize (X14 [] (localenv_nil _) _ _ (type_Sort _ _ Level.prop (localenv_nil _))).
+       specialize (X14 [] localenv_nil _ _ (type_Sort _ _ Level.prop localenv_nil)).
        simpl in X14. forward X14; auto. lia. apply X14.
 
     -- eapply X8; eauto.
@@ -1673,7 +1715,7 @@ Proof.
        eapply (X14 _ wfΓ0 _ _ Hty). lia.
 
     -- eapply X9; eauto.
-       specialize (X14 [] (localenv_nil _) _ _ (type_Sort _ _ Level.prop (localenv_nil _))).
+       specialize (X14 [] localenv_nil _ _ (type_Sort _ _ Level.prop localenv_nil)).
        simpl in X14. forward X14; auto. pose (typing_size_pos H). lia. apply X14.
        unshelve eapply X14; eauto.
 
@@ -1801,129 +1843,165 @@ Ltac my_rename_hyp h th :=
 
 Ltac rename_hyp h ht ::= my_rename_hyp h ht.
 
-(** * Lemmas about All_local_env *)
-
-Lemma nth_error_All_local_env {P Γ n} (isdecl : n < #|Γ|) :
-  All_local_env P Γ ->
-  on_some (on_local_decl P (skipn (S n) Γ)) (nth_error Γ n).
-Proof.
-  induction 1 in n, isdecl |- *. red; simpl.
-  - destruct n; simpl; inv isdecl.
-  - destruct n. red; simpl. red. simpl. apply t0.
-    simpl. apply IHX. simpl in isdecl. lia.
-  - destruct n. auto.
-    apply IHX. simpl in *. lia.
-Qed.
-
-Lemma lookup_on_global_env `{checker_flags} P Σ c decl :
-  on_global_env P Σ ->
-  lookup_env (fst Σ) c = Some decl ->
-  { Σ' & { wfΣ' : on_global_env P Σ' & on_global_decl P Σ' decl } }.
-Proof.
-  induction 1; simpl. congruence.
-  destruct ident_eq. intros [= ->].
-  exists (Σ0, snd Σ). exists X. auto.
-  apply IHX.
-Qed.
-
-Lemma All_local_env_app `{checker_flags}
-      (P : context -> term -> option term -> Type) l l' :
-  All_local_env P (l ,,, l') ->
-  All_local_env P l * All_local_env (fun Γ t T => P (l ,,, Γ) t T) l'.
-Proof.
-  induction l'; simpl; split; auto.
-  - constructor.
-  - unfold app_context in X.
-    inv X.
-    + intuition auto.
-    + apply IHl'. auto.
-  - inv X.
-    + eapply localenv_cons_abs.
-      * apply IHl'. apply X0.
-      * apply X1.
-    + eapply localenv_cons_def.
-      * apply IHl'. apply X0.
-      * apply X1.
-      * apply X2.
-Qed.
-
-Lemma All_local_env_lookup `{checker_flags} {P Γ n} {decl} :
-  All_local_env P Γ ->
-  nth_error Γ n = Some decl ->
-  on_local_decl P (skipn (S n) Γ) decl.
-Proof.
-  induction 1 in n, decl |- *. simpl. destruct n; simpl; congruence.
-  destruct n. red. simpl. intros [= <-]. simpl. apply t0.
-  simpl in *. eapply IHX.
-  destruct n. simpl. intros [= <-]. auto.
-  eapply IHX.
-Qed.
-
-Lemma All_local_env_app_inv `{checker_flags} (P : context -> term -> option term -> Type) l l' :
-  All_local_env P l * All_local_env (fun Γ t T => P (l ,,, Γ) t T) l' ->
-  All_local_env P (l ,,, l').
-Proof.
-  induction l'; simpl; auto. intuition.
-  intuition. destruct a. destruct decl_body.
-  inv b. econstructor; eauto. inv b; econstructor; eauto. Qed.
-
-Lemma All_local_env_map `{checker_flags} (P : context -> term -> option term -> Type) f l :
-  (forall u, f (tSort u) = tSort u) ->
-  All_local_env (fun Γ t T => P (map (map_decl f) Γ) (f t) (option_map f T)) l -> All_local_env P (map (map_decl f) l).
-Proof.
-  intros Hf. induction 1; econstructor; eauto.
-Qed.
-
-Definition property `{checker_flags} :=
-  forall (Σ : global_context) (Γ : context),
-    All_local_env (lift_typing typing Σ) Γ -> forall t T : term, typing Σ Γ t T -> Type.
-
-Definition lookup_wf_local {Γ P} (wfΓ : All_local_env P Γ) (n : nat) (isdecl : n < #|Γ|) :
-  All_local_env P (skipn (S n) Γ).
-Proof.
-  induction wfΓ in n, isdecl |- *; simpl. constructor.
-  cbn -[skipn] in *. destruct n.
-  simpl. exact wfΓ.
-  apply IHwfΓ. auto with arith.
-  destruct n. exact wfΓ.
-  apply IHwfΓ. auto with arith.
-Defined.
-
-Definition lookup_wf_local_decl {Γ P} (wfΓ : All_local_env P Γ) (n : nat)
-           {decl} (eq : nth_error Γ n = Some decl) :
-  ∑ Pskip : All_local_env P (skipn (S n) Γ),
-    on_local_decl P (skipn (S n) Γ) decl.
-Proof.
-  induction wfΓ in n, decl, eq |- *; simpl.
-  - elimtype False. destruct n; depelim eq.
-  - destruct n.
-    + simpl. exists wfΓ. injection eq; intros <-. apply t0.
-    + apply IHwfΓ. auto with arith.
-  - destruct n.
-    + exists wfΓ. injection eq; intros <-. apply t1.
-    + apply IHwfΓ. apply eq.
-Defined.
-
-Definition on_wf_local_decl `{checker_flags} {Σ Γ}
-           (P : forall Σ Γ (wfΓ : wf_local Σ Γ) t T, Σ ;;; Γ |- t : T -> Type)
-           (wfΓ : wf_local Σ Γ) {d} (H : on_local_decl (lift_typing typing Σ) Γ d) :=
-  match d as d' return (on_local_decl (lift_typing typing Σ) Γ d') -> Type with
-  | {| decl_name := na; decl_body := Some b; decl_type := ty |} => fun H => P Σ Γ wfΓ b ty H
-  | {| decl_name := na; decl_body := None; decl_type := ty |} => fun H => P Σ Γ wfΓ _ _ (projT2 H)
-   end H.
 
 From Equations Require Import Equations.
+Section All_local_env.
+  (** * Lemmas about All_local_env *)
 
-Lemma nth_error_All_local_env_over `{checker_flags} {P Σ Γ n decl} (eq : nth_error Γ n = Some decl) {wfΓ : All_local_env (lift_typing typing Σ) Γ} :
-  All_local_env_over typing P Σ Γ wfΓ ->
-  let Γ' := skipn (S n) Γ in
-  let p := lookup_wf_local_decl wfΓ n eq in
-  (All_local_env_over typing P Σ Γ' (projT1 p) * on_wf_local_decl P (projT1 p) (projT2 p))%type.
-Proof.
-  induction 1 in n, decl, eq |- *. simpl.
-  - destruct n; simpl; elimtype False; discriminate eq.
-  - destruct n. cbn [skipn]. noconf eq. split. apply X. simpl. apply p.
-    simpl. apply IHX.
-  - destruct n. noconf eq. simpl. split; auto.
+  Context {cf: checker_flags}.
+
+  Lemma nth_error_All_local_env {P Γ n} (isdecl : n < #|Γ|) :
+    All_local_env P Γ ->
+    on_some (on_local_decl P (skipn (S n) Γ)) (nth_error Γ n).
+  Proof.
+    induction 1 in n, isdecl |- *. red; simpl.
+    - destruct n; simpl; inv isdecl.
+    - destruct n. red; simpl. red. simpl. apply t0.
+      simpl. apply IHX. simpl in isdecl. lia.
+    - destruct n. auto.
+      apply IHX. simpl in *. lia.
+  Qed.
+
+  Lemma lookup_on_global_env P Σ c decl :
+    on_global_env P Σ ->
+    lookup_env (fst Σ) c = Some decl ->
+    { Σ' & { wfΣ' : on_global_env P Σ' & on_global_decl P Σ' decl } }.
+  Proof.
+    induction 1; simpl. congruence.
+    destruct ident_eq. intros [= ->].
+    exists (Σ0, snd Σ). exists X. auto.
     apply IHX.
-Defined.
+  Qed.
+
+  Lemma All_local_env_app (P : context -> term -> option term -> Type) l l' :
+    All_local_env P (l ,,, l') ->
+    All_local_env P l * All_local_env (fun Γ t T => P (l ,,, Γ) t T) l'.
+  Proof.
+    induction l'; simpl; split; auto.
+    - constructor.
+    - unfold app_context in X.
+      inv X.
+      + intuition auto.
+      + apply IHl'. auto.
+    - inv X.
+      + eapply localenv_cons_abs.
+        * apply IHl'. apply X0.
+        * apply X1.
+      + eapply localenv_cons_def.
+        * apply IHl'. apply X0.
+        * apply X1.
+        * apply X2.
+  Qed.
+
+  Definition wf_local_rel_app {Σ Γ1 Γ2 Γ3} :
+    wf_local_rel Σ Γ1 (Γ2 ,,, Γ3)
+    -> wf_local_rel Σ Γ1 Γ2 * wf_local_rel Σ (Γ1 ,,, Γ2) Γ3.
+  Proof.
+    intros HH; apply All_local_env_app in HH.
+    destruct HH as [H1 H2].
+    split. exact H1. eapply All_local_env_impl. exact H2.
+    intros Γ t [] X; cbn in *; now rewrite <- app_context_assoc.
+  Defined.
+
+
+  Lemma All_local_env_lookup {P Γ n} {decl} :
+    All_local_env P Γ ->
+    nth_error Γ n = Some decl ->
+    on_local_decl P (skipn (S n) Γ) decl.
+  Proof.
+    induction 1 in n, decl |- *. simpl. destruct n; simpl; congruence.
+    destruct n. red. simpl. intros [= <-]. simpl. apply t0.
+    simpl in *. eapply IHX.
+    destruct n. simpl. intros [= <-]. auto.
+    eapply IHX.
+  Qed.
+
+  Lemma All_local_env_app_inv (P : context -> term -> option term -> Type) l l' :
+    All_local_env P l * All_local_env (fun Γ t T => P (l ,,, Γ) t T) l' ->
+    All_local_env P (l ,,, l').
+  Proof.
+    induction l'; simpl; auto. intuition.
+    intuition. destruct a. destruct decl_body.
+    inv b. econstructor; eauto. inv b; econstructor; eauto. Qed.
+
+
+  Definition wf_local_rel_app_inv {Σ Γ1 Γ2 Γ3} :
+    wf_local_rel Σ Γ1 Γ2 -> wf_local_rel Σ (Γ1 ,,, Γ2) Γ3
+    -> wf_local_rel Σ Γ1 (Γ2 ,,, Γ3).
+  Proof.
+    intros H1 H2. eapply All_local_env_app_inv.
+    split. assumption.
+    eapply All_local_env_impl. eassumption.
+    intros Γ t []; cbn;
+      now rewrite app_context_assoc. 
+  Defined.
+
+
+  Lemma All_local_env_map (P : context -> term -> option term -> Type) f l :
+    (forall u, f (tSort u) = tSort u) ->
+    All_local_env (fun Γ t T => P (map (map_decl f) Γ) (f t) (option_map f T)) l
+    -> All_local_env P (map (map_decl f) l).
+  Proof.
+    intros Hf. induction 1; econstructor; eauto.
+  Qed.
+
+  Definition property :=
+    forall (Σ : global_context) (Γ : context),
+      All_local_env (lift_typing typing Σ) Γ -> forall t T : term, typing Σ Γ t T -> Type.
+
+  Definition lookup_wf_local {Γ P} (wfΓ : All_local_env P Γ) (n : nat)
+             (isdecl : n < #|Γ|) :
+    All_local_env P (skipn (S n) Γ).
+  Proof.
+    induction wfΓ in n, isdecl |- *; simpl. constructor.
+    cbn -[skipn] in *. destruct n.
+    simpl. exact wfΓ.
+    apply IHwfΓ. auto with arith.
+    destruct n. exact wfΓ.
+    apply IHwfΓ. auto with arith.
+  Defined.
+
+  Definition on_local_decl_glob (P : term -> option term -> Type) d :=
+    match d.(decl_body) with
+    | Some b => P b (Some d.(decl_type))
+    | None => P d.(decl_type) None
+    end.
+
+  Definition lookup_wf_local_decl {Γ P} (wfΓ : All_local_env P Γ) (n : nat)
+             {decl} (eq : nth_error Γ n = Some decl) :
+    ∑ Pskip : All_local_env P (skipn (S n) Γ),
+             on_local_decl_glob (P (skipn (S n) Γ)) decl.
+  Proof.
+    induction wfΓ in n, decl, eq |- *; simpl.
+    - elimtype False. destruct n; depelim eq.
+    - destruct n.
+      + simpl. exists wfΓ. injection eq; intros <-. apply t0.
+      + apply IHwfΓ. auto with arith.
+    - destruct n.
+      + exists wfΓ. injection eq; intros <-. apply t1.
+      + apply IHwfΓ. apply eq.
+  Defined.
+
+  Definition on_wf_local_decl {Σ Γ}
+             (P : forall Σ Γ (wfΓ : wf_local Σ Γ) t T, Σ ;;; Γ |- t : T -> Type)
+             (wfΓ : wf_local Σ Γ) {d} (H : on_local_decl_glob (lift_typing typing Σ Γ) d) :=
+    match d as d' return (on_local_decl_glob (lift_typing typing Σ Γ) d') -> Type with
+    | {| decl_name := na; decl_body := Some b; decl_type := ty |} => fun H => P Σ Γ wfΓ b ty H
+    | {| decl_name := na; decl_body := None; decl_type := ty |} => fun H => P Σ Γ wfΓ _ _ (projT2 H)
+    end H.
+
+
+  Lemma nth_error_All_local_env_over {P Σ Γ n decl} (eq : nth_error Γ n = Some decl) {wfΓ : All_local_env (lift_typing typing Σ) Γ} :
+    All_local_env_over typing P Σ Γ wfΓ ->
+    let Γ' := skipn (S n) Γ in
+    let p := lookup_wf_local_decl wfΓ n eq in
+    (All_local_env_over typing P Σ Γ' (projT1 p) * on_wf_local_decl P (projT1 p) (projT2 p))%type.
+  Proof.
+    induction 1 in n, decl, eq |- *. simpl.
+    - destruct n; simpl; elimtype False; discriminate eq.
+    - destruct n. cbn [skipn]. noconf eq. split. apply X. simpl. apply p.
+      simpl. apply IHX.
+    - destruct n. noconf eq. simpl. split; auto.
+      apply IHX.
+  Defined.
+End All_local_env.
